coq-osiris/examples/proofs/inversion.v
@@ -27,7 +27,16 @@ Class FinIterable G `{Iterable G, ∀ A, Elements A (G A)} := {
 
   complete_elements {A : Type} :
     ∀ (T : G A) (Xs : list A), complete T Xs → Xs ≡ₚ elements T;
-}.
+  }.
+
+
+(* ========================================================================== *)
+(** * Data Structure. *)
+
+(* We formalize a data structure as a type family [G], such that
+   [G A] is representable for every repesentable type [A]. *)
+Class DataStructure (G : Type → Type) :=
+  is_representable A `{Encode A} :> Encode (G A).
 
 
 (* ========================================================================== *)
@@ -35,23 +44,121 @@ Class FinIterable G `{Iterable G, ∀ A, Elements A (G A)} := {
 
 Section iteration_methods.
   Context `{!osirisGS Σ}.
-  Context {G : Type → Type} `{DataStructure Σ G, Iterable G}
-          {A : Type}         `{Encode A} `{Encode (G A)}.
+  Context {G : Type → Type} `{DataStructure G, Iterable G}
+          {A : Type}         `{Encode A}.
 
-  Variables (t : G A).
+  Variables (T : G A).
 
-  Definition isIter (Ψ : iEff Σ) (iter : val) : iProp Σ :=
+  Definition isIter (ψ : iEff Σ) (iter : val) : iProp Σ :=
     ∀ E (I : list A → iProp Σ) (f : val),
       □ (∀ (Xs : list A) (X : A),
-           ⌜ permitted t (Xs ++ [X]) ⌝ -∗
-             I Xs -∗
-                 EWP (call f #X) @ E <| Ψ |> {{ λ _, I (Xs ++ [X]) }})
+           ⌜ permitted T (Xs ++ [X]) ⌝ -∗
+           I Xs -∗
+           EWP (call f #X) @ E <| ψ |> {{ λ _, I (Xs ++ [X]) }})
       -∗
-          I [] -∗
-          EWP (c ← call iter f;
-               call c #t) @ E <| Ψ |> {{ λ _, ∃ Xs, I Xs ∗ ⌜ complete t Xs ⌝ }}.
+      I [] -∗
+      EWP (call iter f) @E <| ψ |> {{ RET c,
+      EWP (call c #T) @ E <| ψ |>
+        {{ λ _, ∃ Xs, I Xs ∗ ⌜ complete T Xs ⌝ }} }}.
 
 End iteration_methods.
+
+(* ------------------------------------------------------------------------ *)
+(** Lift Data Structure. *)
+
+Global Instance lift_data_structure G `{DataStructure G} :
+  DataStructure (G ∘ G).
+Proof. intros ??. simpl. by apply _. Defined.
+
+
+(* ========================================================================== *)
+(** * Lift Iteration Method. *)
+
+Section lift_iteration_method.
+  Context `{!osirisGS Σ}.
+  Context G `{DataStructure G, Iterable G}.
+
+  Definition lift_permitted {A} (TT : (G (G A))) (Xs : list A) : Prop :=
+    (* We match over [last Xs] to facilitate the simplification of
+         assertions of the form [permitted _ (_ ++ [X])]. *)
+    match last Xs with
+    | None => True
+    | _ =>
+        ∃ (Ts : list (G A)) (T : G A) (Xss : list (list A)) (Ys : list A),
+        Xs = concat Xss ++ Ys    ∧
+        permitted TT (Ts ++ [T]) ∧
+        permitted T Ys           ∧
+        Forall2 complete Ts Xss
+  end.
+
+  Definition lift_complete {A} (TT : G (G A)) (Xs : list A) : Prop :=
+    ∃ (Ts : list (G A)) (Xss : list (list A)),
+      Xs = concat Xss         ∧
+        complete TT Ts          ∧
+        Forall2 complete Ts Xss.
+
+  Global Instance lift_iterable : Iterable (G ∘ G) := {
+      permitted := @lift_permitted;
+      complete  := @lift_complete;
+    }.
+
+  (* Value representing [fun f tt -> iter (fun t -> iter f t) tt]. *)
+  Definition lift_iter (iter : val) : val :=
+    (VClo [("iter", iter)]
+            (Anon ("f" =>
+                 EAnonFun
+                   (Anon ("tt" =>
+                            EApp
+                              (EApp
+                                 (EPath ["iter"])
+                                 (EAnonFun (Anon ("t" => EApp (EApp (EPath ["iter"]) (EPath ["f"])) (EPath ["t"])))))
+                              (EPath ["tt"])))))).
+
+  Lemma lift_iter_isIter (iter : val) (Ψ : iEff Σ) :
+      □ (∀ (A : Type) `{Encode A} (T : G A),
+          isIter T Ψ iter)
+        -∗
+      □ (∀ (A : Type) `{Encode A} (TT : (G ∘ G) A),
+          isIter TT Ψ (lift_iter iter)).
+  Proof.
+    iIntros "#Hiter" (????) "!#".
+    iIntros (I f) "#Hf HI". unfold lift_iter.
+    Simp. Ret. Simp. Bind. simpl in *.
+    iApply (ewp_pers_mono with "[HI]").
+    iApply ("Hiter" $!
+              ((* Type of the elements. *) G A) (is_representable A)
+              ((* Data structure. *) TT)
+              ((* Mask. *) E)
+              ((* Invariant. *) λ (Ts : list (G A)), ∃ Xss,
+                  I (concat Xss) ∗ ⌜ Forall2 complete Ts Xss ⌝)%I
+              ((* Iteratee. *) _ )
+             with "[] [HI]"); [|by iExists []; iFrame].
+    - iIntros "!#" (Ts T) "%Hpermitted [%Xss [HI %Hcomplete]]".
+      Simp. Bind.
+      iApply (ewp_pers_mono with "[HI]").
+      iApply ("Hiter" $! A H1 T E
+                ((* Invariant. *) λ (Xs : list A), I (concat Xss ++ Xs))%I
+                ((* Iteratee. *) f)
+               with "[] [HI]"); [|rewrite app_nil_r; by iFrame].
+      + iIntros "!#" (Xs X) "%Hpermitted_T HI".
+        rewrite app_assoc.
+        iApply ("Hf" $! _ X with "[] HI").
+        iPureIntro. rewrite /= /lift_permitted last_app last_cons //=.
+        exists Ts, T, Xss, (Xs ++ [X]).
+        rewrite app_assoc. by repeat split.
+      + iIntros "!#" ([|]); [ simpl | done]; iIntros "Hc !>".
+        iApply (ewp_pers_mono with "Hc").
+        iIntros "!#" (_) "[%Xs [HI %Hcomplete_T]] !>".
+        iExists (Xss ++ [Xs]). rewrite concat_app //= app_nil_r.
+        iFrame. iPureIntro. by decompose_Forall.
+    - iIntros "!#" ([y|]); [ simpl | done]; iIntros "Hc !>".
+      iApply (ewp_pers_mono with "Hc").
+      iIntros "!#" (_) "[%Ts [[%Xss [HI %Hxs]] %Hcomplete_TT]] !>".
+      iExists (concat Xss). iFrame. iPureIntro.
+      rewrite /lift_complete. by exists Ts, Xss.
+    Qed.
+
+End lift_iteration_method.
 
 
 (* ========================================================================== *)
@@ -59,8 +166,8 @@ End iteration_methods.
 
 Section lazy_sequences.
   Context `{!osirisGS Σ}.
-  Context  {G : Type → Type} `{DataStructure Σ G, Iterable G}
-           {A : Type}         `{Encode A} `{Encode (G A)}.
+  Context  {G : Type → Type} `{DataStructure G, Iterable G}
+           {A : Type}         `{Encode A}.
 
   Variables (t : G A).
 
@@ -75,9 +182,9 @@ Section lazy_sequences.
            :  iEff Σ -d> val -d> list A -d> iPropO Σ  :=
     λ Ψ h Xs,
       match h with
-      | VData "None" (VTuple [])       =>
+      | VData "Nil" (VTuple [])       =>
           ⌜ complete t Xs ⌝
-      | VData "Some" p =>
+      | VData "Cons" p =>
           ∃ X k, ⌜ p = #(X, k) ⌝ ∧
                  ⌜ permitted t (Xs ++ [X]) ⌝ ∗ ▷ isSeq Ψ k (Xs ++ [X])
       | _ =>
@@ -128,15 +235,23 @@ Definition yield x : val := VXData yield_eff (VTuple [x]).
 
 Section inversion_protocol.
   Context `{!osirisGS Σ}.
-  Context  {G : Type → Type} `{DataStructure Σ G, Iterable G}.
-  Context {A : Type} `{Encode A}.
+  Context  {G : Type → Type} `{DataStructure G, Iterable G}.
+  Context  {A : Type} `{Encode A}.
 
-  Definition Ψ_yield T (iterView : list A → iProp Σ) : iEff Σ :=
+  Definition ψ_yield T (iterView : list A → iProp Σ) : iEff Σ :=
     (>> Xs X >>
        ! (yield #X)
          {{ iterView Xs ∗ ⌜ permitted T (Xs ++ [X]) ⌝ }};
-       ? (O2Ret #())
+       ? (@O2Ret val exn #())
          {{ iterView (Xs ++ [X]) }} @ OS).
+
+  Lemma upcl_yield T iterView v Φ :
+    iEff_car (upcl OS (ψ_yield T iterView)) v Φ ⊣⊢
+      (∃ Xs (X : A), ⌜ v = yield #X ⌝ ∗
+                             (iterView Xs ∗
+                             ⌜ permitted T (Xs ++ [X]) ⌝) ∗
+                             (iterView (Xs ++ [X]) -∗ Φ (O2Ret (VUnit))))%I.
+  Proof. by rewrite /ψ_yield  (upcl_tele' [tele _ _] [tele]) //=. Qed.
 
 End inversion_protocol.
 
@@ -204,29 +319,235 @@ Section verification.
 
   Section specification.
     Context `{!osirisGS Σ}.
-    Context {G : Type → Type} `{DataStructure Σ G, Iterable G}.
+    Context {G : Type → Type} `{DataStructure G, Iterable G}.
     Context {A : Type}         `{Encode A} `{Encode (G A)}.
 
     (* ------------------------------------------------------------------------ *)
     (** Specification of [invert]. *)
 
-    (* [λ f, iter f t] *)
-    Definition itere :=
-      EAnonFun
-        (AnonFun
-           "f"
-           (EApp
-              (EApp
-                 (EPath ["iter"])
-                 (EPath ["f"]))
-              (EPath ["t"]))).
+    (* ∀ iter t, iterv iter t ≜ [fun f -> iter f t]. *)
+    Definition iterv iter t :=
+      VClo [("iter", iter); ("t", t)]
+        (Anon ("f" => EApp
+                       (EApp
+                          (EPath ["iter"])
+                          (EPath ["f"]))
+                       (EPath ["t"]))).
+
+    Definition env := ("Yield", (VLoc yield_eff)) :: stdlib_env.
 
     Definition invert_spec invert : iProp Σ :=
-      ∀ (t : G A) (iter : val),
-      isIter t ⊥ iter -∗
-      EWP (iterv ← eval [("iter", #iter); ("t", #t)] itere;
-           call invert iterv) {{ lift_ret_spec (λ k, isSeq t ⊥ k []) }}.
+      ∀ (T : G A) (iter : val),
+      (∀ ψ, isIter T ψ iter) -∗
+      EWP (call_anonfun env invert [(iterv iter #T); #()])
+        {{ lift_ret_spec (λ k, isSeq T ⊥ k []) }}.
 
   End specification.
+
+
+  Section invert_correct.
+    Context `{!osirisGS Σ}.
+    Context  {G : Type → Type} `{DataStructure G, Iterable G}
+             {A : Type}         `{Encode A}.
+    Context `{!inG Σ (excl_authR (leibnizO (list A)))}.
+
+
+    Ltac get_outcome_from_match e :=
+    lazymatch e with
+    | (pre_eval_match_aux _ _ _ ?o _ _) => constr:(o)
+    | (deep_handler_body _ ?o _ _) => constr:(o)
+    | (shallow_handler_body _ ?o _ _) => constr:(o)
+    end.
+    Ltac trivial_post_instantiation :=
+      lazymatch goal with
+      | |- envs_entails _ ?G =>
+          lazymatch G with
+          | ewp_def _ ?e _ _ =>
+              lazymatch (get_outcome_from_match e) with
+              | O3Ret _ => constr:(True)
+              | O3Throw _ => constr:(True)
+              | O3Perform _ _ => constr:(True \/ True)
+              end
+          end
+      end.
+    Ltac skip_matching_branch :=
+      let φ2 := trivial_post_instantiation in
+      iApply (handle_cons _ _ _ _ _ _ _ _ _ (λ _, False) φ2);
+      [ specify_cpattern; pattern_match
+      | iIntros (? [])
+      | iIntros (_) ].
+    Ltac skip_non_matching_branch :=
+      iApply handle_cons_skip; [ reflexivity | ].
+    Ltac skip_branch :=
+      (skip_non_matching_branch || skip_matching_branch);
+      fold deep_handler_body; fold shallow_handler_body.
+    Ltac enter_branch :=
+      iApply (handle_cons with "[-]");
+      [ specify_cpattern; pattern_match; try (apply eq_refl)
+      | (iIntros (? ->) || iIntros (? <-))
+      | let F := fresh in iIntros (F); tauto ].
+
+    (* Try to reduce a [match] expression by skipping all branches seen and then
+     entering a branch on match. *)
+    Ltac red_match := repeat (skip_branch; [ idtac ]); enter_branch.
+
+    Ltac ewp_call_anonfun :=
+      (* Unfold [call_anonfun], and get a tower of binds. *)
+      rewrite /call_anonfun; simpl; rewrite ?bind_bind;
+      (* Unfold [eval_anonfun]. *)
+      rewrite /eval_anonfun;
+      (* Simplify the tower of binds,
+        this should elaborate a closure capturing all arguments.  *)
+      repeat (iApply ewp_bind; Simp; Ret);
+      simpl.
+
+    (* Non-recursive call. *)
+    Ltac Call :=
+      match goal with
+      | |- envs_entails _ (ewp_def _ (call_anonfun _ _ _) _ _) =>
+          ewp_call_anonfun; iApply ewp_call_nonrec
+      end.
+
+    Definition invert := __fun9.
+
+    Definition ieq {PROP : bi} {A : Type} y := λ (x : A), @bi_pure PROP (x = y).
+
+    Lemma yield_handler_correct (iter : val) γ (Ys : list A) (T : G A) :
+      handlerView γ Ys -∗
+      deep_handler_spec ⊤ (ψ_yield T (iterView γ))
+        (λ _ : outcome2 val exn, ∃ Xs : list A, iterView γ Xs ∗ ⌜complete T Xs⌝)
+        (λ o : code.outcome3 val exn,
+            deep_handler_body
+              ("__osiris_anonymous_arg" ~> VUnit;
+               "yield" ~> VClo ("iter" ~> iterv iter #T;
+                                "__osiris_anonymous_arg" ~> iterv iter #T;
+                                env) __fun0;
+               "iter" ~> iterv iter #T;
+               "__osiris_anonymous_arg" ~> iterv iter #T;
+               env) o __branches3 __branches3) ⊥ (RET h, isHead T ⊥ h Ys).
+    Proof.
+      iLöb as "IH" forall (Ys γ).
+      iIntros "HhandlerView".
+      rewrite deep_handler_spec_unfold /deep_handler_spec_pre.
+      iSplit.
+      { iIntros (o) "[%Xs [HiterView %Hcomplete]]".
+        iPoseProof (confront_views with "HhandlerView HiterView") as "->".
+        iModIntro.
+        destruct o; red_match;
+          with_strategy transparent [evals] Simp; Ret;
+          by iPureIntro. }
+
+      { iIntros (v k) "HProt".
+        rewrite /prot; iPoseProof (upcl_yield with "HProt") as "HProt".
+        iDestruct "HProt" as "[%Xs [%X [-> [[HiterView %Hpermitted] HProt]]]]".
+        iModIntro.
+        iPoseProof (confront_views with "HhandlerView HiterView") as "->".
+        iApply ewp_fupd. iMod (update_cell γ (Ys ++ [X]) with "HhandlerView HiterView")
+          as "[HhandlerView HiterView]"; iModIntro.
+        red_match.
+        with_strategy transparent [evals] Simp. Ret. simpl.
+        iExists _, _. iSplit; [ iPureIntro; reflexivity | ]. iSplit; [ by iPureIntro | ].
+        iModIntro.
+        rewrite !isSeq_unfold /isSeq_pre.
+        with_strategy transparent [extend] Simp.
+        Bind. rewrite /as_cont. Bind. Simp. Ret. Bind.
+        with_strategy transparent [evals] Simp. Ret. simpl.
+        iApply ("HProt" with "HiterView").
+        iModIntro.
+        iSpecialize ("IH" $! (Ys ++ [X]) γ with "HhandlerView").
+        rewrite /deep_handler_spec seal_eq.
+        iApply "IH". }
+    Qed.
+
+   Lemma ewp_invert : ⊢ @invert_spec _ _ G _ _ A _ _ invert. simpl.
+      iIntros (T iter) "Hiter".
+      iApply ewp_fupd.
+      iMod (new_cell []) as (γ) "[HhandlerView HiterView]"; iModIntro.
+
+      rewrite /call_anonfun; simpl; rewrite ?bind_bind.
+      rewrite /eval_anonfun.
+      iApply ewp_bind. Simp. Ret. simpl.
+      iApply ewp_bind.
+
+      iApply ewp_call_nonrec.
+      iApply ewp_EMatch.
+      iApply (ewp_deep_handler _ ⊥ (ieq ?[y])).
+
+      { Simp. by Ret. }
+
+      rewrite /ieq.
+
+      rewrite deep_handler_spec_unfold; iSplit; last first.
+      (* Effectful case: we don't allow effect (TODO: automate). *)
+      { iModIntro. iIntros (??) "HF".
+        by iPoseProof (upcl_bottom with "HF") as "F". }
+
+      iModIntro. iIntros (? ->). iModIntro.
+      enter_branch.
+
+      (* [let open struct ...] *)
+      iApply ewp_ELetOpen.
+      with_strategy transparent [eval_mexpr] Ret. simpl.
+      iExists _; iSplit; [ done | ].
+
+      (* [let yield x = ...] *)
+      iApply (ewp_ELet_singleton_total (ieq ?[y])).
+      { Simp. by Ret. }
+      iIntros (? ->).
+      iExists _; iSplit.
+      { iPureIntro.
+        eapply prove_simp_try.
+        { with_strategy transparent [extend] apply SimpReflexive. }
+        apply SimpReflexive. }
+
+      (* fun () -> match iter yield with ... *)
+      Simp. Ret. simpl.
+
+      iApply ewp_call_nonrec.
+      iModIntro.
+      iApply ewp_EMatch.
+      iApply (ewp_deep_handler _ _ (ieq ?[y])).
+
+      { Simp. by Ret. }
+
+      rewrite /__branches4. rewrite !/deco.
+      rewrite deep_handler_spec_unfold; iSplit; last first.
+      { iIntros (??) "HF".
+        by iPoseProof (upcl_bottom with "HF") as "F". }
+      iIntros (? ->). iModIntro.
+
+      enter_branch.
+
+      (* [match_with iter yield { ...] *)
+      iApply ewp_EMatch.
+      iApply (ewp_pers_mono _ _ ((lift_ret_spec (λ h, isHead T ⊥ h []))) with "[-]").
+      iApply (ewp_deep_handler
+                (* E: *)
+                ⊤
+                (* Handlee's protocol: *)
+                (ψ_yield T (iterView γ))
+                (* Handlee's postcondition: *)
+                (λ _, ∃ (Xs : list A), iterView γ Xs ∗ ⌜ complete T Xs ⌝)%I
+                (* Handler's protocol: *)
+                ⊥
+                (* Handler's postcondition: *)
+                (lift_ret_spec (λ h, isHead T ⊥ h [])) with "[Hiter HiterView] [HhandlerView]").
+
+      { Simp. Bind.
+        iApply (ewp_pers_mono with "[-]").
+        { iApply ("Hiter" with "[] HiterView").
+          iIntros "!#" (Xs X) "%Hpermitted HI".
+          with_strategy transparent [evals] Simp.
+          iApply ewp_perform.
+          rewrite /prot. iApply upcl_yield.
+          iExists _, _.
+          iSplit; [ equality | ]. iFrame. iSplit; [ by iPureIntro | by iIntros "?" ]. }
+        iIntros "!#" ([|]); [ by iIntros "?" | done ]. }
+
+      { iApply (yield_handler_correct with "HhandlerView"). }
+
+      { iIntros "!#" ([|]); [ simpl | done ].
+        iIntros "HisHead !>".
+        rewrite isSeq_unfold /isSeq_pre isHead_unfold /isHead_pre.
 
 End verification.
